Main.lean
@@ -1,4 +1,72 @@
-import ArchSem
+import Cli
+import ArchSem.LitmusTest.Parse
+import ArchSem.LitmusTest.Run
+import ArchSem.TerminatingModel
+import ArchSemTinyArm.Promising
 
-def main : IO Unit :=
-  IO.println s!"Hello, {hello}!"
+open ArchSem.LitmusTest
+open ArchSem.TerminatingModel (ComputationalTerminatingModel)
+
+def modelFromStr (fuel : Nat) : String → Option ComputationalTerminatingModel
+  | "tinyarm-promisefirst" =>
+    ArchSemTinyArm.Promising.createPromiseFirstModel
+      ArchSemTinyArm.sailTinyArmIsem fuel |> some
+  | "tinyarm-promisenaive" =>
+    ArchSemTinyArm.Promising.createNaiveModel
+      ArchSemTinyArm.sailTinyArmIsem fuel |> some
+  | _ => none
+
+-- TODO: terminal colors.
+def runTests (p : Cli.Parsed) : IO UInt32 := do
+  let testFnames : List System.FilePath := p.variableArgsAs! String |>.toList
+  if testFnames.length == 0 then
+    IO.eprintln s!"No tests specified."
+    return 1
+  let fuel : Nat ← match p.flag? "fuel" |>.bind (Cli.Parsed.Flag.as? · Nat) with
+    | .some fuel => pure fuel
+    | .none =>
+      IO.eprintln s!"Fuel must be Nat."
+      return 1
+  let modelStr : String ← match p.flag? "model" |>.bind (Cli.Parsed.Flag.as? · String) with
+    | .some str => pure str
+    | .none =>
+      IO.eprintln s!"Model unspecified."
+      return 1
+  let model ← match modelFromStr fuel modelStr with
+    | .some m => pure m
+    | .none => do
+      IO.eprintln s!"Model does not exist: '{modelStr}'"
+      return 1
+  let tests : List TestRepr ← testFnames.mapM Parse.readTestFile
+  let passed : List Bool ← List.zipWithM (fun fname test => do
+    let result : Except String Unit := Run.runLitmusTest model test
+    match result with
+    | .ok () =>
+      IO.print s!"[ PASS ] ({fname})\n"
+      pure true
+    | .error msg =>
+      IO.print s!"[ FAIL ] ({fname}):\n{msg}\n"
+      pure false
+  ) testFnames tests
+  if passed.all (· == true) then
+    IO.println "✔ All tests passed."
+    pure 0
+  else
+    IO.println "✘ At least one test failed."
+    pure 1
+
+
+def litmusTestCmd : Cli.Cmd := `[Cli|
+  archsem VIA runTests;
+  "Run litmus tests from `.archsem.toml` format."
+
+  FLAGS:
+    model : String; "Name of model to use."
+    fuel : Nat; ""
+
+  ARGS:
+    ...tests : String; "Tests to run of the `.archsem.toml` format."
+]
+
+def main (args : List String) : IO UInt32 :=
+  litmusTestCmd.validate args
